LogicalRefinement/Denot/Wk.lean
@@ -323,66 +323,48 @@ theorem HasType.wk_eq
     | @union Δ' A B _ _ IA IB =>
       dsimp only [Term.denote_ty]
       simp only [pure]
+      apply existential_forall_helper_dep (by rw [Term.stlc_ty_wk]);
+      intro x;
       apply congr (congr rfl _) _;
       {
-        --TODO: clean this mess up...
-        simp only [Ne]
-        apply arrow_equivalence _ rfl;
-        apply propext; apply Iff.intro;
-        {
-          intro Ha; rw [Ha]; exact interp_eq_none
-        }
-        {
-          intro Ha;
-          cases a with
-          | none => rfl
-          | some a => rw [interp_eq_some] at Ha; contradiction
-        }
+        rw [IA R rfl]
+        rw [rec_to_cast']
+        rw [rec_to_cast']
       }
       {
-        apply existential_forall_helper_dep (by rw [Term.stlc_ty_wk]);
-        intro x;
-        apply congr (congr rfl _) _;
+        rw [@IB 
+          ((Hyp.mk _ (HypKind.val type))::Γ) 
+          _ _ _ (x, G) R.lift rfl];            
+        apply congr (congr rfl _) rfl;
+        rw [<-Stlc.Context.interp.wk_lift]
+        let Δ'' := Term.stlc_ty A :: Context.stlc (Context.upgrade Δ');
+        let f: 
+          (Γ: Stlc.Context) -> Γ.interp 
+          -> Stlc.WkCtx ρ.lift Γ Δ'' -> (Stlc.Context.interp Δ'')
+          := λΓ => @Stlc.Context.interp.wk Γ Δ'' ρ.lift;
+        have Hf: ∀Γ, @Stlc.Context.interp.wk Γ Δ'' ρ.lift = f Γ 
+          := by intros; rfl;
+        rw [Hf]
+        rw [Hf]
+        apply cast_app_dep_two f;
+        rfl
         {
-          rw [IA R rfl]
-          rw [rec_to_cast']
-          rw [rec_to_cast']
+          simp only [
+            Context.upgrade, Hyp.upgrade, A.stlc_ty_wk, Context.stlc
+          ]
         }
         {
-          rw [@IB 
-            ((Hyp.mk _ (HypKind.val type))::Γ) 
-            _ _ _ (x, G) R.lift rfl];            
-          apply congr (congr rfl _) rfl;
-          rw [<-Stlc.Context.interp.wk_lift]
-          let Δ'' := Term.stlc_ty A :: Context.stlc (Context.upgrade Δ');
-          let f: 
-            (Γ: Stlc.Context) -> Γ.interp 
-            -> Stlc.WkCtx ρ.lift Γ Δ'' -> (Stlc.Context.interp Δ'')
-            := λΓ => @Stlc.Context.interp.wk Γ Δ'' ρ.lift;
-          have Hf: ∀Γ, @Stlc.Context.interp.wk Γ Δ'' ρ.lift = f Γ 
-            := by intros; rfl;
-          rw [Hf]
-          rw [Hf]
-          apply cast_app_dep_two f;
-          rfl
+          rw [cast_pair']
           {
-            simp only [
-              Context.upgrade, Hyp.upgrade, A.stlc_ty_wk, Context.stlc
-            ]
-          }
-          {
-            rw [cast_pair']
             {
-              {
-                apply congr (congr rfl _) rfl;
-                rw [A.stlc_ty_wk]
-                rw [rec_to_cast']
-                rw [cast_merge]
-                rfl
-              }
+              apply congr (congr rfl _) rfl;
+              rw [A.stlc_ty_wk]
+              rw [rec_to_cast']
+              rw [cast_merge]
+              rfl
             }
-            rfl
           }
+          rfl
         }
       }
     | @dimplies Δ' A B _ _ IA IB => 
